theories/Dot/examples/scalaLib.v
@@ -1,0 +1,214 @@
+From stdpp Require Import strings.
+
+From D Require Import tactics.
+From D.Dot Require Import syn exampleInfra unstampedness_binding.
+From D.Dot.typing Require Import typing_unstamped typing_unstamped_derived.
+
+Implicit Types (L T U: ty) (v: vl) (e: tm) (d: dm) (ds: dms) (Γ : list ty).
+
+(** * Infinite loops *)
+Definition loopDefV : vl := ν {@ (* self => *)
+  val "loop" = vabs (tapp (tproj (tv x1) "loop") (tv x0))
+  (* λ v, self.loop v. *)
+}.
+Definition loopDefTConcr : ty := μ {@ val "loop" : ⊤ →: ⊥ }.
+Definition loopDefT : ty := val "loop" : ⊤ →: ⊥.
+Example loopDefTyp Γ : Γ u⊢ₜ tv loopDefV : loopDefT.
+Proof.
+  apply (Subs_typed_nocoerce loopDefTConcr).
+  - tcrush; cbv.
+    eapply App_typed; last var. tcrush.
+    varsub. cbv. lThis.
+  - apply Bind1; tcrush.
+Qed.
+
+Definition loopTm := tapp (tproj (tv loopDefV) "loop") (tv (vnat 0)).
+Example loopTyp Γ : Γ u⊢ₜ loopTm : ⊥.
+Proof.
+  pose proof loopDefTyp Γ.
+  apply (App_typed (T1 := ⊤)); tcrush.
+  apply (Subs_typed_nocoerce 𝐍); tcrush.
+Qed.
+
+(** * Booleans, Church-encoded. *)
+(** Sec. 5 of WadlerFest DOT.
+IFTFun ≡ { if: ∀(x: {A: ⊥..⊤})∀(t: x.A)∀(f: x.A): x.A }
+IFT ≡ { if: IFTFun }
+
+let boolImpl =
+ν (b: { Boolean: IFT..IFT } ∧ { true: IFT } ∧ { false: IFT })
+{ Boolean = IFT } ∧
+{ true = λ(x: {A: ⊥..⊤})λ(t: x.A)λ(f: x.A)t } ∧ { false = λ(x: {A: ⊥..⊤})λ(t: x.A)λ(f: x.A)f }
+
+In fact, that code doesn't typecheck as given, and we fix it by setting.
+
+IFT ≡ IFTFun
+let bool = boolImpl : μ { Boolean: IFT..IFT; true : b.Boolean; false : b.Boolean }
+ *)
+Definition IFTBody : ty := p0 @; "A" →: p0 @; "A" →: p0 @; "A".
+Definition IFT : ty :=
+  TAll (tparam "A") IFTBody.
+
+(* Definition IFT : ty := {@ val "if" : IFTFun }. *)
+
+Definition iftTrue := vabs (vabs' (vabs' (tv x1))).
+Definition iftFalse := vabs (vabs' (vabs' (tv x0))).
+
+Example iftTrueTyp Γ : Γ u⊢ₜ tv iftTrue : IFT.
+Proof. tcrush. var. Qed.
+Example iftFalseTyp Γ : Γ u⊢ₜ tv iftFalse : IFT.
+Proof. tcrush. var. Qed.
+
+Definition boolImpl :=
+  ν {@
+    type "Boolean" = IFT;
+    val "true" = iftTrue;
+    val "false" = iftFalse
+  }.
+
+Definition boolImplTConcr : ty :=
+  μ {@
+    typeEq "Boolean" IFT;
+    val "true" : IFT;
+    val "false" : IFT
+  }.
+
+Definition p0Bool := p0 @; "Boolean".
+
+(* This type makes "Boolean" nominal by abstracting it. *)
+Definition boolImplT : ty :=
+  μ {@
+    type "Boolean" >: ⊥ <: IFT;
+    val "true" : TLater p0Bool;
+    val "false" : TLater p0Bool
+  }.
+
+Example SubIFT_P0Bool Γ : {@
+    typeEq "Boolean" IFT;
+    val "true" : IFT;
+    val "false" : IFT
+  }%ty :: Γ u⊢ₜ IFT, 0 <: p0Bool, 0.
+Proof. eapply LSel_stp'; tcrush. varsub; tcrush. Qed.
+
+Example SubIFT_LaterP0Bool' Γ : {@
+    typeEq "Boolean" IFT;
+    val "true" : IFT;
+    val "false" : IFT
+  }%ty :: Γ u⊢ₜ IFT, 0 <: ▶ p0Bool, 0.
+Proof. eapply Trans_stp; first exact: SubIFT_P0Bool. tcrush. Qed.
+
+Example SubIFT_LaterP0Bool Γ : (▶ {@
+    typeEq "Boolean" IFT;
+    val "true" : ▶ p0Bool;
+    val "false" : ▶ p0Bool
+  })%ty :: Γ u⊢ₜ IFT, 0 <: ▶ p0Bool, 0.
+Proof.
+  asideLaters.
+  eapply Trans_stp; first (apply (AddI_stp _ _ 1); tcrush).
+  eapply LSel_stp'; tcrush.
+  varsub; tcrush.
+Qed.
+
+Example boolImplTypConcr Γ :
+  Γ u⊢ₜ tv boolImpl : boolImplTConcr.
+Proof. tcrush; by [apply (dty_typed IFT); tcrush | var]. Qed.
+
+Example boolImplTyp Γ :
+  Γ u⊢ₜ tv boolImpl : boolImplT.
+Proof.
+  apply (Subs_typed_nocoerce boolImplTConcr); first by apply boolImplTypConcr.
+  tcrush; rewrite iterate_0.
+  - lThis.
+  - lNext.
+    lThis.
+    apply SubIFT_LaterP0Bool'.
+  - do 2 lNext.
+    lThis.
+    apply SubIFT_LaterP0Bool'.
+Qed.
+
+(*
+  Encoding Option. Beware I'm using raw Church-encoded booleans, simply
+    because it's easier.
+  type Option = {
+    type T
+    val isEmpty: Boolean
+    val pmatch: [U] => U => (T => U) => U
+  }
+*)
+
+Definition optionT : ty := μ {@ (* self => *)
+  tparam "T";
+  val "isEmpty" : IFT;
+  val "pmatch" : TAll (tparam "U") (p0 @; "U" →: (p1 @; "T" →: p0 @; "U") →: p0 @; "U")
+  (* ∀ x : {type U}, x.U → (self.T -> x.U) -> x.U *)
+}.
+(*
+  type None = Option { type T = Nothing }
+  def mkNone[T]: None = new {
+    type T = Nothing
+    val isEmpty = true
+    val pmatch: [U] => U => (T => U) => U = [U] => (none: U) => (some: T => U) => none
+  }
+*)
+Definition noneT0 := TAnd optionT ({@ typeEq "T" ⊥}).
+Definition noneT : ty := μ {@ (* self => *)
+  typeEq "T" ⊥;
+  val "isEmpty" : IFT;
+  val "pmatch" : TAll (tparam "U") (p0 @; "U" →: (p1 @; "T" →: p0 @; "U") →: p0 @; "U")
+}.
+Definition mkNone : vl := ν {@
+  type "T" = ⊥;
+  val "isEmpty" = iftTrue;
+  val "pmatch" = vabs (vabs' (vabs' (tv x1)))
+}.
+
+Example noneTyp Γ :
+  Γ u⊢ₜ tv mkNone : noneT.
+Proof.
+  (* apply VObj_typed; last stcrush.
+  apply dcons_typed; [tcrush| |tcrush].
+  apply dcons_typed; [eauto using iftTrueTyp| |tcrush]. *)
+  tcrush; var.
+Qed.
+
+(*
+  //type Some = Option & { self => val get: self.T }
+  type Some = Option & { type T; val get: T }
+  def mkSome[S](t: S): Some { type T = S } = new {
+    type T = S
+    val isEmpty = false
+    val get = t
+    val pmatch: [U] => U => (T => U) => U = [U] => (none: U) => (some: T => U) => some(get)
+  }
+*)
+
+Definition someT T : ty := μ {@ (* self => *)
+  typeEq "T" (shift T);
+  val "isEmpty" : IFT;
+  val "pmatch" : TAll (tparam "U") (p0 @; "U" →: (p1 @; "T" →: p0 @; "U") →: p0 @; "U");
+  val "get" : ▶ p0 @; "T"
+}.
+Definition mkSomeT : ty := TAll (tparam "A") (p0 @; "A" →: someT (p0 @; "A")).
+Definition mkSome : tm := vabs' $ vabs' $ tv $ ν {@
+  type "T" = p2 @; "A";
+  val "isEmpty" = iftFalse;
+  val "pmatch" = vabs (vabs' (vabs' (tapp (tv x0) (tskip (tproj (tv x3) "get")))));
+  val "get" = x1
+}.
+
+Example mkSomeTyp Γ :
+  Γ u⊢ₜ mkSome : mkSomeT.
+Proof.
+  tcrush; first var; cbv; hideCtx.
+  - eapply App_typed; first var.
+    rewrite -(iterate_S tskip 0);
+      apply (Subs_typed (T1 := (▶ (p3 @; "T"))%ty)); tcrush.
+    varsub.
+    repeat lNext.
+  - varsub.
+    eapply Trans_stp; first (apply TAddLater_stp; tcrush).
+    asideLaters.
+    eapply LSel_stp'; tcrush.
+    varsub; tcrush.
+Qed.
